Additions to simple patricia tree theory.
* should now EVAL in good time
* union proved correct
* fold characterised a bit
* domain defined

src/patricia/sptreeScript.sml
@@ -1,8 +1,27 @@
 open HolKernel Parse boolLib bossLib;
 open lcsymtacs
 open arithmeticTheory
+open logrootTheory
 
 val _ = new_theory "sptree";
+
+(* A log-time random-access, extensible array implementation with union.
+
+   The "array" can be gappy: there don't have to be elements at any
+   particular index, and, being a finite thing, there is obviously a
+   maximum index past which there are no elements at all. It is
+   possible to update at an index past the current maximum index. It
+   is also possible to delete values at an index.
+
+   Should EVAL well. Big drawback is that there doesn't seem to be an
+   efficient way to do an in index-order traversal of the elements.
+   There is a fold function that gives you access to all the key-value
+   pairs, but these will come out in an inconvenient order.
+
+   The insert, delete and union operations all preserve a
+   well-formedness condition ("wf") that ensures there is only one
+   possible representation for any given finite-map.
+*)
 
 val _ = Datatype`spt = LN | LS 'a | BN spt spt | BS spt 'a spt`
 (* Leaf-None, Leaf-Some, Branch-None, Branch-Some *)
@@ -18,18 +37,19 @@ val wf_def = Define`
   (wf (BS t1 a t2) <=> wf t1 /\ wf t2 /\ ~(isEmpty t1 /\ isEmpty t2))
 `
 
-val lookup_def = tDefine "lookup" `
-  (lookup n LN = NONE) /\
-  (lookup n (LS a) = if n = 0 then SOME a else NONE) /\
-  (lookup n (BN t1 t2) =
-     if n = 0 then NONE
-     else lookup ((n - 1) DIV 2) (if EVEN n then t1 else t2)) /\
-  (lookup n (BS t1 a t2) =
-     if n = 0 then SOME a
-     else lookup ((n - 1) DIV 2) (if EVEN n then t1 else t2))
+fun tzDefine s q = Lib.with_flag (computeLib.auto_import_definitions,false) (tDefine s q)
+val lookup_def = tzDefine "lookup" `
+  (lookup k LN = NONE) /\
+  (lookup k (LS a) = if k = 0 then SOME a else NONE) /\
+  (lookup k (BN t1 t2) =
+     if k = 0 then NONE
+     else lookup ((k - 1) DIV 2) (if EVEN k then t1 else t2)) /\
+  (lookup k (BS t1 a t2) =
+     if k = 0 then SOME a
+     else lookup ((k - 1) DIV 2) (if EVEN k then t1 else t2))
 ` (WF_REL_TAC `measure FST` >> simp[DIV_LT_X])
 
-val insert_def = tDefine "insert" `
+val insert_def = tzDefine "insert" `
   (insert k a LN = if k = 0 then LS a
                      else if EVEN k then BN (insert ((k-1) DIV 2) a LN) LN
                      else BN LN (insert ((k-1) DIV 2) a LN)) /\
@@ -133,16 +153,175 @@ val union_def = Define`
        | BS t1' a' t2' => BS (union t1 t1') a (union t2 t2'))
 `;
 
+val isEmpty_union = store_thm(
+  "isEmpty_union",
+  ``isEmpty (union m1 m2) <=> isEmpty m1 /\ isEmpty m2``,
+  map_every Cases_on [`m1`, `m2`] >> simp[union_def, isEmpty_def]);
+
+val wf_union = store_thm(
+  "wf_union",
+  ``!m1 m2. wf m1 /\ wf m2 ==> wf (union m1 m2)``,
+  Induct >> simp[wf_def, union_def] >>
+  Cases_on `m2` >> simp[wf_def,isEmpty_union] >>
+  metis_tac[]);
+
+val optcase_lemma = prove(
+  ``(case opt of NONE => NONE | SOME v => SOME v) = opt``,
+  Cases_on `opt` >> simp[]);
+
+val lookup_union = store_thm(
+  "lookup_union",
+  ``!m1 m2 k. lookup k (union m1 m2) =
+              case lookup k m1 of
+                NONE => lookup k m2
+              | SOME v => SOME v``,
+  Induct >> simp[lookup_def] >- simp[union_def] >>
+  Cases_on `m2` >> simp[lookup_def, union_def] >>
+  rw[optcase_lemma]);
+
+val lrnext_def = new_specification(
+  "lrnext_def", ["lrnext"],
+  numeralTheory.bit_initiality
+      |> INST_TYPE [alpha |-> ``:num``]
+      |> Q.SPECL [`1`, `\n r. 2 * r`,
+                  `\n r. 2 * r`]
+      |> SIMP_RULE bool_ss []);
+val lrnext' = prove(
+  ``(!a. lrnext 0 = 1) /\ (!n a. lrnext (NUMERAL n) = lrnext n)``,
+  simp[NUMERAL_DEF, GSYM ALT_ZERO, lrnext_def])
+val lrnext_thm = save_thm(
+  "lrnext_thm",
+  LIST_CONJ (CONJUNCTS lrnext' @ CONJUNCTS lrnext_def))
+val _ = computeLib.add_persistent_funs ["lrnext_thm"]
+
+val domain_def = Define`
+  (domain LN = {}) /\
+  (domain (LS _) = {0}) /\
+  (domain (BN t1 t2) =
+     IMAGE (\n. 2 * n + 2) (domain t1) UNION
+     IMAGE (\n. 2 * n + 1) (domain t2)) /\
+  (domain (BS t1 _ t2) =
+     {0} UNION IMAGE (\n. 2 * n + 2) (domain t1) UNION
+     IMAGE (\n. 2 * n + 1) (domain t2))
+`;
+val _ = export_rewrites ["domain_def"]
+
+val FINITE_domain = store_thm(
+  "FINITE_domain",
+  ``FINITE (domain t)``,
+  Induct_on `t` >> simp[]);
+val _ = export_rewrites ["FINITE_domain"]
+
+val bit_cases = prove(
+  ``!n. (n = 0) \/ (?m. n = 2 * m + 1) \/ (?m. n = 2 * m + 2)``,
+  Induct >> simp[] >> fs[]
+  >- (disj1_tac >> qexists_tac `0` >> simp[])
+  >- (disj2_tac >> qexists_tac `m` >> simp[])
+  >- (disj1_tac >> qexists_tac `SUC m` >> simp[]))
+
+val oddevenlemma = prove(
+  ``2 * y + 1 <> 2 * x + 2``,
+  disch_then (mp_tac o AP_TERM ``EVEN``) >>
+  simp[EVEN_ADD, EVEN_MULT]);
+
+val MULT2_DIV' = prove(
+  ``(2 * m DIV 2 = m) /\ ((2 * m + 1) DIV 2 = m)``,
+  simp[DIV_EQ_X]);
+
+val domain_lookup = store_thm(
+  "domain_lookup",
+  ``!t k. k IN domain t <=> ?v. lookup k t = SOME v``,
+  Induct >> simp[domain_def, lookup_def] >> rpt gen_tac >>
+  qspec_then `k` STRUCT_CASES_TAC bit_cases >>
+  simp[oddevenlemma, EVEN_ADD, EVEN_MULT,
+       EQ_MULT_LCANCEL, MULT2_DIV']);
+
+val lookup_NONE_domain = store_thm(
+  "lookup_NONE_domain",
+  ``(lookup k t = NONE) <=> k NOTIN domain t``,
+  simp[domain_lookup] >> Cases_on `lookup k t` >> simp[]);
+
 val foldi_def = Define`
   (foldi f i acc LN = acc) /\
   (foldi f i acc (LS a) = f i a acc) /\
   (foldi f i acc (BN t1 t2) =
-     foldi f (2 * i + 1) (foldi f (2 * i + 2) acc t1) t2) /\
+     let inc = lrnext i
+     in
+       foldi f (i + inc) (foldi f (i + 2 * inc) acc t1) t2) /\
   (foldi f i acc (BS t1 a t2) =
-     foldi f (2 * i + 1) (f i a (foldi f (2 * i + 2) acc t1)) t2)
+     let inc = lrnext i
+     in
+       foldi f (i + inc) (f i a (foldi f (i + 2 * inc) acc t1)) t2)
 `;
 
-val toList_def = Define`toList = foldi (\k v a. CONS v a) 0 []`
+val lrnext212 = prove(
+  ``(lrnext (2 * m + 1) = 2 * lrnext m) /\
+    (lrnext (2 * m + 2) = 2 * lrnext m)``,
+  conj_tac >| [
+    `2 * m + 1 = BIT1 m` suffices_by simp[lrnext_thm] >>
+    simp_tac bool_ss [BIT1, TWO, ONE, MULT_CLAUSES, ADD_CLAUSES],
+    `2 * m + 2 = BIT2 m` suffices_by simp[lrnext_thm] >>
+    simp_tac bool_ss [BIT2, TWO, ONE, MULT_CLAUSES, ADD_CLAUSES]
+  ]);
+
+val bit_induction = prove(
+  ``!P. P 0 /\ (!n. P n ==> P (2 * n + 1)) /\
+        (!n. P n ==> P (2 * n + 2)) ==>
+        !n. P n``,
+  gen_tac >> strip_tac >> completeInduct_on `n` >> simp[] >>
+  qspec_then `n` strip_assume_tac bit_cases >> simp[]);
+
+val lrlemma1 = prove(
+  ``lrnext (i + lrnext i) = 2 * lrnext i``,
+  qid_spec_tac `i` >> ho_match_mp_tac bit_induction >>
+  simp[lrnext212, lrnext_thm] >> conj_tac
+  >- (gen_tac >>
+      `2 * i + (2 * lrnext i + 1) = 2 * (i + lrnext i) + 1`
+         by decide_tac >> simp[lrnext212]) >>
+  qx_gen_tac `i` >>
+  `2 * i + (2 * lrnext i + 2) = 2 * (i + lrnext i) + 2`
+    by decide_tac >>
+  simp[lrnext212]);
+
+val lrlemma2 = prove(
+  ``lrnext (i + 2 * lrnext i) = 2 * lrnext i``,
+  qid_spec_tac `i` >> ho_match_mp_tac bit_induction >>
+  simp[lrnext212, lrnext_thm] >> conj_tac
+  >- (qx_gen_tac `i` >>
+      `2 * i + (4 * lrnext i + 1) = 2 * (i + 2 * lrnext i) + 1`
+        by decide_tac >> simp[lrnext212]) >>
+  gen_tac >>
+  `2 * i + (4 * lrnext i + 2) = 2 * (i + 2 * lrnext i) + 2`
+     by decide_tac >> simp[lrnext212])
+
+val set_foldi_keys = store_thm(
+  "set_foldi_keys",
+  ``!t a i. foldi (\k v a. k INSERT a) i a t =
+            a UNION IMAGE (\n. i + lrnext i * n) (domain t)``,
+  Induct_on `t` >> simp[foldi_def, GSYM pred_setTheory.IMAGE_COMPOSE,
+                        combinTheory.o_ABS_R]
+  >- simp[Once pred_setTheory.INSERT_SING_UNION, pred_setTheory.UNION_COMM]
+  >- (simp[pred_setTheory.EXTENSION] >> rpt gen_tac >>
+      Cases_on `x IN a` >> simp[lrlemma1, lrlemma2, LEFT_ADD_DISTRIB]) >>
+  simp[pred_setTheory.EXTENSION] >> rpt gen_tac >>
+  Cases_on `x IN a'` >> simp[lrlemma1, lrlemma2, LEFT_ADD_DISTRIB])
+
+val domain_foldi = save_thm(
+  "domain_foldi",
+  set_foldi_keys |> SPEC_ALL |> Q.INST [`i` |-> `0`, `a` |-> `{}`]
+                 |> SIMP_RULE (srw_ss()) [lrnext_thm]
+                 |> SYM);
+
+val _ = remove_ovl_mapping "lrnext" {Name = "lrnext", Thy = "sptree"}
+
+val toListA_def = Define`
+  (toListA acc LN = acc) /\
+  (toListA acc (LS a) = a::acc) /\
+  (toListA acc (BN t1 t2) = toListA (toListA acc t2) t1) /\
+  (toListA acc (BS t1 a t2) = toListA (a :: toListA acc t2) t1)
+`;
+val toList_def = Define`toList m = toListA [] m`
+
 val numeral_div0 = prove(
   ``(BIT1 n DIV 2 = n) /\
     (BIT2 n DIV 2 = SUC n) /\
@@ -175,7 +354,7 @@ val BITDIV = prove(
   ``((BIT1 n - 1) DIV 2 = n) /\ ((BIT2 n - 1) DIV 2 = n)``,
   simp[PRE_BIT1, PRE_BIT2] >> simp[DIV_EQ_X]);
 
-fun computerule rwts th q =
+fun computerule th q =
     th
       |> CONJUNCTS
       |> map SPEC_ALL
@@ -186,23 +365,38 @@ fun computerule rwts th q =
                                        numTheory.NOT_SUC, BITDIV,
                                        EVAL ``SUC 0 DIV 2``,
                                        numeralTheory.numeral_evenodd,
-                                       EVEN] @ rwts))))
+                                       EVEN]) THENC
+                            SIMP_CONV bool_ss [ALT_ZERO])))
+
+val lookup_compute = save_thm(
+  "lookup_compute",
+    LIST_CONJ (prove (``lookup (NUMERAL n) t = lookup n t``,
+                      REWRITE_TAC [NUMERAL_DEF]) ::
+               computerule lookup_def `0` @
+               computerule lookup_def `ZERO` @
+               computerule lookup_def `BIT1 n` @
+               computerule lookup_def `BIT2 n`))
+val _ = computeLib.add_persistent_funs ["lookup_compute"]
 
 val insert_compute = save_thm(
   "insert_compute",
     LIST_CONJ (prove (``insert (NUMERAL n) a t = insert n a t``,
                       REWRITE_TAC [NUMERAL_DEF]) ::
-               computerule [] insert_def `0` @
-               computerule [] insert_def `BIT1 n` @
-               computerule [] insert_def `BIT2 n`))
+               computerule insert_def `0` @
+               computerule insert_def `ZERO` @
+               computerule insert_def `BIT1 n` @
+               computerule insert_def `BIT2 n`))
+val _ = computeLib.add_persistent_funs ["insert_compute"]
 
 val delete_compute = save_thm(
   "delete_compute",
     LIST_CONJ (
       prove(``delete (NUMERAL n) t = delete n t``,
             REWRITE_TAC [NUMERAL_DEF]) ::
-      computerule [] delete_def `0` @
-      computerule [] delete_def `BIT1 n` @
-      computerule [] delete_def `BIT2 n`))
+      computerule delete_def `0` @
+      computerule delete_def `ZERO` @
+      computerule delete_def `BIT1 n` @
+      computerule delete_def `BIT2 n`))
+val _ = computeLib.add_persistent_funs ["delete_compute"]
 
 val _ = export_theory();
